SyntaxMacros.v
@@ -1,20 +1,20 @@
 Require Import Coq.Lists.List.
-Require Import SGA.Syntax SGA.Primitives SGA.Interop.
+Require Import SGA.Syntax SGA.TypedSyntax SGA.Primitives SGA.Interop.
 Import ListNotations.
 
 Section SyntaxMacros.
-  Context {pos_t var_t reg_t: Type}.
+  Context {pos_t method_name_t var_t reg_t: Type}.
 
   Section ConstBits.
     Context {fn_t: Type}.
-    Notation uaction := (uaction pos_t var_t reg_t fn_t).
+    Notation uaction := (uaction pos_t method_name_t var_t reg_t fn_t).
 
     Definition UConstBits {sz} (bs: bits sz) : uaction :=
       UConst (tau := bits_t sz) bs.
   End ConstBits.
 
   Context {custom_fn_t: Type}.
-  Notation uaction := (uaction pos_t var_t reg_t (interop_ufn_t custom_fn_t)).
+  Notation uaction := (uaction pos_t method_name_t var_t reg_t (interop_ufn_t custom_fn_t)).
 
   Definition USkip : uaction :=
     UConstBits Ob.
@@ -62,3 +62,85 @@ Section SyntaxMacros.
     List.fold_left (fun acc '(f, a) => UCall (usubst f) acc a)
                    fields (UCall uinit (UConstBits Ob) (UConstBits Ob)).
 End SyntaxMacros.
+
+Section TypedSyntaxMacros.
+  Context {var_t reg_t fn_t: Type}.
+  Context {R: reg_t -> type}
+          {Sigma: fn_t -> ExternalSignature}.
+
+  Notation action := (action var_t R Sigma).
+
+  Fixpoint mshift {K} (prefix: list K) {sig: list K} {k} (m: member k sig)
+    : member k (prefix ++ sig) :=
+    match prefix return member k sig -> member k (prefix ++ sig) with
+    | [] => fun m => m
+    | k' :: prefix => fun m => MemberTl k k' (prefix ++ sig) (mshift prefix m)
+    end m.
+
+  Fixpoint mshift' {K} (infix: list K) {sig sig': list K} {k} (m: member k (sig ++ sig'))
+    : member k (sig ++ infix ++ sig').
+  Proof.
+    destruct sig as [ | k' sig].
+    - exact (mshift infix m).
+    - destruct (mdestruct m) as [(-> & Heq) | (m' & Heq)]; cbn in *.
+      + exact (MemberHd k' (sig ++ infix ++ sig')).
+      + exact (MemberTl k k' (sig ++ infix ++ sig') (mshift' _ infix sig sig' k m')).
+  Defined.
+
+  Fixpoint infix_action (infix: tsig var_t) {sig sig': tsig var_t} {tau} (a: action (sig ++ sig') tau)
+    : action (sig ++ infix ++ sig') tau.
+  Proof.
+    remember (sig ++ sig'); destruct a; subst.
+    - exact (Fail tau).
+    - exact (Var (mshift' infix m)).
+    - exact (Const cst).
+    - exact (Assign (mshift' infix m) (infix_action infix _ _ _ a)).
+    - exact (Seq (infix_action infix _ _ _ a1) (infix_action infix _ _ _ a2)).
+    - exact (Bind var (infix_action infix _ _ _ a1) (infix_action infix (_ :: sig) sig' _ a2)).
+    - exact (If (infix_action infix _ _ _ a1) (infix_action infix _ _ _ a2) (infix_action infix _ _ _ a3)).
+    - exact (Read port idx).
+    - exact (Write port idx (infix_action infix _ _ _ a)).
+    - exact (Call fn (infix_action infix _ _ _ a1) (infix_action infix _ _ _ a2)).
+  Defined.
+
+  Definition prefix_action (prefix: tsig var_t) {sig: tsig var_t} {tau} (a: action sig tau)
+    : action (prefix ++ sig) tau :=
+    infix_action prefix (sig := []) a.
+
+  Fixpoint suffix_action_eqn {A} (l: list A) {struct l}:
+    l ++ [] = l.
+  Proof. destruct l; cbn; [ | f_equal ]; eauto. Defined.
+
+  Definition suffix_action (suffix: tsig var_t) {sig: tsig var_t} {tau} (a: action sig tau)
+    : action (sig ++ suffix) tau.
+  Proof. rewrite <- (suffix_action_eqn suffix); apply infix_action; rewrite (suffix_action_eqn sig); exact a. Defined.
+
+  Fixpoint InternalCall'
+           {tau: type}
+           (sig: tsig var_t)
+           (fn_sig: tsig var_t)
+           (fn_body: action (fn_sig ++ sig) tau)
+           (args: context (fun '(_, tau) => action sig tau) fn_sig)
+    : action sig tau :=
+    match fn_sig return action (fn_sig ++ sig) tau ->
+                        context (fun '(_, tau) => action sig tau) fn_sig ->
+                        action sig tau with
+    | [] =>
+      fun fn_body _ =>
+        fn_body
+    | (k, tau) :: fn_sig =>
+      fun fn_body args =>
+        InternalCall' sig fn_sig
+                      (Bind k (prefix_action fn_sig (chd args)) fn_body)
+                      (ctl args)
+    end fn_body args.
+
+  Fixpoint InternalCall
+             {tau: type}
+             (sig: tsig var_t)
+             (fn_sig: tsig var_t)
+             (fn_body: action fn_sig tau)
+             (args: context (fun '(_, tau) => action sig tau) fn_sig)
+    : action sig tau :=
+    InternalCall' sig fn_sig (suffix_action sig fn_body) args.
+End TypedSyntaxMacros.
